theories/logrel_heaplang/ltyping_safety.v
@@ -9,9 +9,6 @@ Lemma ltyped_safety `{heapPreG Σ} e σ es σ' e' :
 Proof.
   intros Hty. apply (heap_adequacy Σ NotStuck e σ (λ _, True))=> // ?.
   destruct (Hty _) as [A He]. iStartProof. iDestruct (He $! ∅) as "#He".
-  iSpecialize ("He" with "[]").
-  { iSplit.
-    - iPureIntro=> x. rewrite !lookup_empty -!not_eq_None_Some. by naive_solver.
-    - by rewrite map_zip_with_empty. }
+  iSpecialize ("He" with "[]"); first by rewrite /env_ltyped.
   rewrite subst_map_empty. iApply (wp_wand with "He"); auto.
 Qed.
